Translation/SAst.v
@@ -32,6 +32,7 @@ Inductive sterm : Type :=
 | sCongLambda (B1 B2 t1 t2 pA pB pt : sterm)
 | sCongApp (B1 B2 pu pA pB pv : sterm)
 | sCongSum (B1 B2 pA pB : sterm)
+| sCongPair (B1 B2 pA pB pu pv : sterm)
 | sCongPi1 (B1 B2 pA pB pp : sterm)
 | sCongPi2 (B1 B2 pA pB pp : sterm)
 | sCongEq (pA pu pv : sterm)
