Translation/Translation.v
@@ -102,6 +102,23 @@ Proof.
   - apply type_Eq ; assumption.
 Defined.
 
+Definition trans_subst {Σ Γ s A B u Γ' A' B' u'} :
+  type_glob Σ ->
+  Σ |--i Γ' # ⟦ Γ ⟧ ->
+  Σ ;;;; Γ',, A' |--- [B']: sSort s # ⟦ Γ,, A |--- [B]: sSort s ⟧ ->
+  Σ ;;;; Γ' |--- [u']: A' # ⟦ Γ |--- [u]: A ⟧ ->
+  Σ ;;;; Γ' |--- [B'{ 0 := u' }]: sSort s # ⟦ Γ |--- [B{ 0 := u }]: sSort s ⟧.
+Proof.
+  intros hg hΓ hB hu.
+  destruct hΓ.
+  destruct hB as [[[? ?] ?] ?]. destruct hu as [[[? ?] ?] ?].
+  repeat split.
+  - assumption.
+  - constructor.
+  - apply inrel_subst ; assumption.
+  - lift_sort. eapply typing_subst ; eassumption.
+Defined.
+
 (* Maybe put this together with the other translation definitions *)
 Definition eqtrans Σ Γ A u v Γ' A' A'' u' v' p' :=
   Γ ⊂ Γ' *
@@ -129,6 +146,8 @@ Defined.
 Scheme typing_ind := Induction for XTyping.typing Sort Type
   with wf_ind := Induction for XTyping.wf Sort Type
   with eq_term_ind := Induction for XTyping.eq_term Sort Type.
+
+(* Set Printing Depth 100. *)
 
 (* Combined Scheme typing_all from typing_ind , wf_ind , eq_term_ind. *)
 
@@ -189,6 +208,17 @@ Definition typing_all : forall (Σ : sglobal_context)
              P (Γ,, t) b (sSort s2) t1 ->
              P Γ (sSum n t b) (sSort (max_sort s1 s2))
                (XTyping.type_Sum Σ Γ n t b s1 s2 t0 t1)) ->
+       (forall (Γ : scontext) (n : name) (A B u v : sterm) (s1 s2 : sort)
+          (t : Σ;;; Γ |-x A : sSort s1),
+        P Γ A (sSort s1) t ->
+        forall t0 : Σ;;; Γ,, A |-x B : sSort s2,
+        P (Γ,, A) B (sSort s2) t0 ->
+        forall t1 : Σ;;; Γ |-x u : A,
+        P Γ u A t1 ->
+        forall t2 : Σ;;; Γ |-x v : B {0 := u},
+        P Γ v (B {0 := u}) t2 ->
+        P Γ (sPair A B u v) (sSum n A B)
+          (XTyping.type_Pair Σ Γ n A B u v s1 s2 t t0 t1 t2)) ->
        (forall (Γ : scontext) (n : name) (A B : sterm) (s1 s2 : sort) (p : sterm)
           (t : Σ;;; Γ |-x p : sSum n A B),
            P Γ p (sSum n A B) t ->
@@ -319,6 +349,29 @@ Definition typing_all : forall (Σ : sglobal_context)
         P (Γ,, A2) B2 (sSort s2) t0 ->
         P1 Γ (sSum n1 A1 B1) (sSum n2 A2 B2) (sSort (max_sort s1 s2))
            (XTyping.cong_Sum Σ Γ n1 n2 A1 A2 B1 B2 s1 s2 e e0 t t0)) ->
+       (forall (Γ : scontext) (n : name) (A1 A2 B1 B2 u1 u2 v1 v2 : sterm)
+          (s1 s2 : sort) (e : Σ;;; Γ |-x A1 = A2 : sSort s1),
+        P1 Γ A1 A2 (sSort s1) e ->
+        forall e0 : Σ;;; Γ,, A1 |-x B1 = B2 : sSort s2,
+        P1 (Γ,, A1) B1 B2 (sSort s2) e0 ->
+        forall e1 : Σ;;; Γ |-x u1 = u2 : A1,
+        P1 Γ u1 u2 A1 e1 ->
+        forall e2 : Σ;;; Γ |-x v1 = v2 : B1 {0 := u1},
+        P1 Γ v1 v2 (B1 {0 := u1}) e2 ->
+        forall t : Σ;;; Γ,, A1 |-x B1 : sSort s2,
+        P (Γ,, A1) B1 (sSort s2) t ->
+        forall t0 : Σ;;; Γ,, A2 |-x B2 : sSort s2,
+        P (Γ,, A2) B2 (sSort s2) t0 ->
+        forall t1 : Σ;;; Γ |-x u1 : A1,
+        P Γ u1 A1 t1 ->
+        forall t2 : Σ;;; Γ |-x u2 : A2,
+        P Γ u2 A2 t2 ->
+        forall t3 : Σ;;; Γ |-x v1 : B1 {0 := u1},
+        P Γ v1 (B1 {0 := u1}) t3 ->
+        forall t4 : Σ;;; Γ |-x v2 : B2 {0 := u2},
+        P Γ v2 (B2 {0 := u2}) t4 ->
+        P1 Γ (sPair A1 B1 u1 v1) (sPair A2 B2 u2 v2) (sSum n A1 B1)
+          (XTyping.cong_Pair Σ Γ n A1 A2 B1 B2 u1 u2 v1 v2 s1 s2 e e0 e1 e2 t t0 t1 t2 t3 t4)) ->
        (forall (Γ : scontext) (nx ny : name) (A1 A2 B1 B2 : sterm) (s1 s2 : sort)
           (p1 p2 : sterm) (e : Σ;;; Γ |-x p1 = p2 : sSum nx A1 B1),
         P1 Γ p1 p2 (sSum nx A1 B1) e ->
@@ -405,7 +458,7 @@ Proof.
            {Γ'} (hΓ : Σ |--i Γ' # ⟦ Γ ⟧),
            ∑ A' A'' u' v' p',
          eqtrans Σ Γ A u v Γ' A' A'' u' v' p')
-      _ _ _ _ _ _ _ _ _ _ _ _ _ _ _ _ _ _ _ _ _ _ _ _ _ _ _
+      _ _ _ _ _ _ _ _ _ _ _ _ _ _ _ _ _ _ _ _ _ _ _ _ _ _ _ _ _
    ) ; intros.
   (** context_translation **)
 
@@ -549,6 +602,42 @@ Proof.
       (* Now we conclude *)
       exists (sSort (max_sort s1 s2)), (sSum n t'' b'').
       now apply trans_Sum.
+
+    (* type_Pair *)
+    + (* Translation of the domain *)
+      destruct (H _ hΓ) as [S' [A'' hA'']].
+      assert (th : type_head (head (sSort s1))) by constructor.
+      destruct (choose_type hg th hA'') as [T' [[A' hA'] hh]].
+      clear hA'' A'' S'.
+      destruct T' ; inversion hh.
+      subst. clear hh th.
+      (* Translation of the codomain *)
+      destruct (H0 _ (trans_snoc hΓ hA'))
+        as [S' [B'' hB'']].
+      assert (th : type_head (head (sSort s2))) by constructor.
+      destruct (choose_type hg th hB'') as [T' [[B' hB'] hh]].
+      clear hB'' B'' S'.
+      destruct T' ; inversion hh. subst. clear hh th.
+      (* Translation of the first component *)
+      destruct (H1 _ hΓ) as [A'' [u'' hu'']].
+      destruct (change_type hg hu'' hA') as [u' hu'].
+      clear hu'' A'' u''.
+      (* Translation of the second component *)
+      destruct (H2 _ hΓ) as [Bv' [v'' hv'']].
+      destruct (change_type hg hv'' (trans_subst hg hΓ hB' hu')) as [v' hv'].
+      clear hv'' Bv' v''.
+      (* Now we conclude *)
+      exists (sSum n A' B'), (sPair A' B' u' v').
+      destruct hΓ.
+      destruct hA' as [[[? ?] ?] ?].
+      destruct hB' as [[[? ?] ?] ?].
+      destruct hu' as [[[? ?] ?] ?].
+      destruct hv' as [[[? ?] ?] ?].
+      repeat split.
+      * assumption.
+      * constructor ; assumption.
+      * constructor ; assumption.
+      * eapply type_Pair' ; eassumption.
 
     (* type_Pi1 *)
     + (* Translation of the domain *)
@@ -1805,6 +1894,284 @@ Proof.
       cbn in hp5. rewrite <- llift_substProj, <- rlift_substProj in hp5.
       rewrite !llift00, !rlift00 in hp5.
       apply hp5.
+
+    (* cong_Pair *)
+    + (* The domains *)
+      destruct (H _ hΓ)
+        as [T1 [T2 [A1'' [A2'' [pA h1']]]]].
+      destruct (eqtrans_trans hg h1') as [hA1'' hA2''].
+      destruct h1' as [[[[[? ?] ?] ?] ?] hpA''].
+      assert (th : type_head (head (sSort s1))) by constructor.
+      destruct (choose_type hg th hA1'') as [T' [[A1' hA1'] hh]].
+      destruct T' ; inversion hh. subst.
+      clear hh.
+      destruct (choose_type hg th hA2'') as [T' [[A2' hA2'] hh]].
+      destruct T' ; inversion hh. subst.
+      clear hh th.
+      (* Now the codomains *)
+      destruct (H0 _ (trans_snoc hΓ hA1'))
+        as [S1 [S2 [B1'' [B2'' [pB h2']]]]].
+      destruct (eqtrans_trans hg h2') as [hB1'' hB2''].
+      assert (th : type_head (head (sSort s2))) by constructor.
+      destruct (choose_type hg th hB1'') as [T' [[B1' hB1'] hh]].
+      destruct T' ; inversion hh. subst.
+      clear hh.
+      destruct (choose_type hg th hB2'') as [T' [[B2' hB2'] hh]].
+      destruct T' ; inversion hh. subst.
+      clear hh th.
+      destruct h2' as [[[[[? ?] ?] ?] ?] hpB''].
+      (* Now we connect the paths for the domains *)
+      assert (hq1 : ∑ p1, Σ ;;; Γ' |-i p1 : sHeq (sSort s1) A1' (sSort s1) A2').
+      { destruct hA1' as [[_ eA1'] hA1'].
+        destruct hA1'' as [_ hA1''].
+        destruct hA2' as [[_ eA2'] hA2'].
+        destruct hA2'' as [_ hA2''].
+        assert (hr : A1' ∼ A1'').
+        { eapply trel_trans.
+          - eapply trel_sym. eapply inrel_trel. eassumption.
+          - eapply inrel_trel. eassumption.
+        }
+        destruct (trel_to_heq Γ' hg hr) as [pl hpl].
+        specialize (hpl _ _ ltac:(eassumption) ltac:(eassumption)).
+        assert (hr' : A2'' ∼ A2').
+        { eapply trel_trans.
+          - eapply trel_sym. eapply inrel_trel. eassumption.
+          - eapply inrel_trel. eassumption.
+        }
+        destruct (trel_to_heq Γ' hg hr') as [pr hpr].
+        specialize (hpr _ _ ltac:(eassumption) ltac:(eassumption)).
+        exists (sHeqTrans (sHeqTrans pl pA) pr).
+        eapply type_HeqTrans' ; try assumption.
+        - eapply type_HeqTrans' ; eassumption.
+        - eassumption.
+      }
+      destruct hq1 as [q1 hq1].
+      (* And then the paths for the codomains *)
+      pose (Γ1 := nil ,, A1').
+      pose (Γ2 := nil ,, A2').
+      pose (Γm := [ sPack A1' A2' ]).
+      assert (hm : ismix Σ Γ' Γ1 Γ2 Γm).
+      { revert Γm.
+        replace A1' with (llift0 #|@nil sterm| A1')
+          by (cbn ; now rewrite llift00).
+        replace A2' with (rlift0 #|@nil sterm| A2')
+          by (cbn ; now rewrite rlift00).
+        intros.
+        destruct hA1' as [[? ?] ?].
+        destruct hA2' as [[? ?] ?].
+        econstructor.
+        - constructor.
+        - eassumption.
+        - assumption.
+      }
+      pose (Δ := Γ' ,,, Γm).
+      assert (hq2 : ∑ q2, Σ ;;; Γ' ,,, Γ1 |-i q2 : sHeq (sSort s2) B1'
+                                                       (sSort s2) B2').
+      { destruct hB1' as [[_ eB1'] hB1'].
+        destruct hB1'' as [_ hB1''].
+        destruct hB2' as [[_ eB2'] hB2'].
+        destruct hB2'' as [_ hB2''].
+        assert (hr : B1' ∼ B1'').
+        { eapply trel_trans.
+          - eapply trel_sym. eapply inrel_trel. eassumption.
+          - eapply inrel_trel. eassumption.
+        }
+        destruct (trel_to_heq (Γ',, A1') hg hr) as [pl hpl].
+        specialize (hpl _ _ ltac:(eassumption) ltac:(eassumption)).
+        assert (hr' : B2'' ∼ B2').
+        { eapply trel_trans.
+          - eapply trel_sym. eapply inrel_trel. eassumption.
+          - eapply inrel_trel. eassumption.
+        }
+        destruct (trel_to_heq (Γ',, A1') hg hr') as [pr hpr].
+        specialize (hpr _ _ ltac:(eassumption) ltac:(eassumption)).
+        exists (sHeqTrans (sHeqTrans pl pB) pr).
+        eapply type_HeqTrans' ; try assumption.
+        - eapply type_HeqTrans' ; eassumption.
+        - eassumption.
+      }
+      destruct hq2 as [q2 hq2].
+      assert (hp3 : ∑ p3, Σ ;;; Δ |-i p3 : sHeq (sSort s2)
+                                               (llift0 #|Γm| B1')
+                                               (sSort s2)
+                                               (llift0 #|Γm| B2')
+             ).
+      { exists (llift0 #|Γm| q2).
+        match goal with
+        | |- _ ;;; _ |-i _ : ?T =>
+          change T with (llift0 #|Γm| (sHeq (sSort s2) B1' (sSort s2) B2'))
+        end.
+        eapply type_llift0 ; try easy.
+      }
+      destruct hp3 as [p3 hp3].
+      (* Also translating the typing hypothesis for B2 *)
+      destruct (H4 _ (trans_snoc hΓ hA2'))
+        as [S' [B2''' hB2''']].
+      assert (th : type_head (head (sSort s2))) by constructor.
+      destruct (choose_type hg th hB2''') as [T' [[tB2 htB2] hh]].
+      clear hB2''' B2''' S'.
+      destruct T' ; inversion hh. subst. clear hh th.
+      (* Now we can use the strong version of the lemma to build a path between
+         B2' and tB2 !
+       *)
+      assert (hp4 : ∑ p4, Σ ;;; Δ |-i p4 : sHeq (sSort s2) (llift0 #|Γm| B2')
+                                               (sSort s2) (rlift0 #|Γm| tB2)
+             ).
+      { change (sSort s2) with (llift0 #|Γm| (sSort s2)) at 1.
+        change (sSort s2) with (rlift0 #|Γm| (sSort s2)) at 2.
+        assert (hr : B2' ∼ tB2).
+        { destruct htB2 as [[? ?] ?].
+          destruct hB2' as [[? ?] ?].
+          eapply trel_trans.
+          + eapply trel_sym. eapply inrel_trel. eassumption.
+          + apply inrel_trel. assumption.
+        }
+        edestruct (trel_to_heq' hg hr) as [p4 hp4].
+        exists p4. apply hp4.
+        - eassumption.
+        - destruct hB2' as [[? ?] ?]. assumption.
+        - destruct htB2 as [[? ?] ?]. assumption.
+      }
+      destruct hp4 as [p4 hp4].
+      (* This gives us a better path *)
+      assert (hp5 : ∑ p5, Σ ;;; Δ |-i p5 : sHeq (sSort s2) (llift0 #|Γm| B1')
+                                               (sSort s2) (rlift0 #|Γm| tB2)
+             ).
+      { exists (sHeqTrans p3 p4).
+        eapply type_HeqTrans' ; eassumption.
+      }
+      destruct hp5 as [p5 hp5].
+      (* Cleaning *)
+      clear hp4 p4 hp3 p3 hq2 q2.
+      clear hB2' B2' hB2'' hpB'' hB1'' hpA'' hA1'' hA2''.
+      (* clear i8 i7 i6 i5 i4 S1 S2 B1'' B2'' pB. *)
+      (* clear i3 i2 i1 i0 i T1 T2 A1'' A2'' pA. *)
+      clear pA pB pi2_1 pi2_2 A1'' A2''.
+      rename q1 into pA, p5 into pB, hq1 into hpA, hp5 into hpB.
+      rename tB2 into B2', htB2 into hB2'.
+      (* We can now translate the first components. *)
+      destruct (H1 _ hΓ)
+        as [P1 [P1' [u1'' [u2'' [pt h3']]]]].
+      destruct (eqtrans_trans hg h3') as [hu1'' hu2''].
+      destruct (change_type hg hu1'' hA1') as [u1' hu1'].
+      destruct (change_type hg hu2'' hA1') as [u2' hu2'].
+      destruct h3' as [[[[[? ?] ?] ?] ?] hpu].
+      destruct (H6 _ hΓ)
+        as [P2 [u2''' hu2''']].
+      destruct (change_type hg hu2''' hA2') as [tu2 htu2].
+      clear hu2''' u2''' P2.
+      assert (hqt : ∑ qt,
+        Σ ;;; Γ' |-i qt : sHeq A1' u1' A2' tu2
+      ).
+      { destruct hu1'' as [[[? ?] ?] ?].
+        destruct hu2'' as [[[? ?] ?] ?].
+        destruct hu1' as [[[? ?] ?] ?].
+        destruct hu2' as [[[? ?] ?] ?].
+        destruct htu2 as [[[? ?] ?] ?].
+        assert (r1 : u1' ∼ u1'').
+        { eapply trel_trans.
+          - eapply trel_sym. eapply inrel_trel. eassumption.
+          - apply inrel_trel. assumption.
+        }
+        destruct (trel_to_heq Γ' hg r1) as [pl hpl].
+        specialize (hpl _ _ ltac:(eassumption) ltac:(eassumption)).
+        assert (r2 : u2'' ∼ tu2).
+        { eapply trel_trans.
+          - eapply trel_sym. eapply inrel_trel. eassumption.
+          - apply inrel_trel. assumption.
+        }
+        destruct (trel_to_heq Γ' hg r2) as [pr hpr].
+        specialize (hpr _ _ ltac:(eassumption) ltac:(eassumption)).
+        exists (sHeqTrans pl (sHeqTrans pt pr)).
+        eapply type_HeqTrans' ; try assumption.
+        - eassumption.
+        - eapply type_HeqTrans' ; eassumption.
+      }
+      destruct hqt as [qt hqt].
+      (* We can now translate the second components. *)
+      destruct (H2 _ hΓ)
+        as [Q1 [Q1' [v1'' [v2'' [pt' h3']]]]].
+      destruct (eqtrans_trans hg h3') as [hv1'' hv2''].
+      destruct (change_type hg hv1'' (trans_subst hg hΓ hB1' hu1'))
+        as [v1' hv1'].
+      destruct (change_type hg hv2'' (trans_subst hg hΓ hB1' hu1'))
+        as [v2' hv2'].
+      destruct h3' as [[[[[? ?] ?] ?] ?] hpv].
+      destruct (H8 _ hΓ)
+        as [Q2 [v2''' hv2''']].
+      destruct (change_type hg hv2''' (trans_subst hg hΓ hB2' htu2))
+        as [tv2 htv2].
+      clear hv2''' v2''' Q2.
+      assert (hqt' : ∑ qt,
+        Σ ;;; Γ' |-i qt : sHeq (B1'{0 := u1'}) v1' (B2'{0 := tu2}) tv2
+      ).
+      { destruct hv1'' as [[[? ?] ?] ?].
+        destruct hv2'' as [[[? ?] ?] ?].
+        destruct hv1' as [[[? ?] ?] ?].
+        destruct hv2' as [[[? ?] ?] ?].
+        destruct htv2 as [[[? ?] ?] ?].
+        assert (r1 : v1' ∼ v1'').
+        { eapply trel_trans.
+          - eapply trel_sym. eapply inrel_trel. eassumption.
+          - apply inrel_trel. assumption.
+        }
+        destruct (trel_to_heq Γ' hg r1) as [pl hpl].
+        specialize (hpl _ _ ltac:(eassumption) ltac:(eassumption)).
+        assert (r2 : v2'' ∼ tv2).
+        { eapply trel_trans.
+          - eapply trel_sym. eapply inrel_trel. eassumption.
+          - apply inrel_trel. assumption.
+        }
+        destruct (trel_to_heq Γ' hg r2) as [pr hpr].
+        specialize (hpr _ _ ltac:(eassumption) ltac:(eassumption)).
+        exists (sHeqTrans pl (sHeqTrans pt' pr)).
+        eapply type_HeqTrans' ; try assumption.
+        - eassumption.
+        - eapply type_HeqTrans' ; eassumption.
+      }
+      destruct hqt' as [qt' hqt'].
+      (* We have an equality between Pairs now *)
+      assert (hpi : ∑ qpi,
+        Σ ;;; Γ' |-i qpi : sHeq (sSum n A1' B1') (sPair A1' B1' u1' v1')
+                               (sSum n A2' B2') (sPair A2' B2' tu2 tv2)
+      ).
+      { exists (sCongPair B1' B2' pA pB qt qt').
+        destruct hB1' as [[[? ?] ?] ?].
+        destruct hB2' as [[[? ?] ?] ?].
+        eapply type_CongPair' ; try eassumption.
+        cbn in hpB. rewrite <- llift_substProj, <- rlift_substProj in hpB.
+        rewrite !llift00, !rlift00 in hpB.
+        apply hpB.
+      }
+      destruct hpi as [qpi hpi].
+      (* Finally we translate the right Pair to put it in the left Sum *)
+      rename e into eA.
+      pose (e := sHeqTypeEq (sSum n A2' B2') (sSum n A1' B1') (sHeqSym qpi)).
+      pose (tpi := sTransport (sSum n A2' B2') (sSum n A1' B1') e (sPair A2' B2' tu2 tv2)).
+      (* We conclude *)
+      exists (sSum n A1' B1'), (sSum n A1' B1').
+      exists (sPair A1' B1' u1' v1'), tpi.
+      exists (sHeqTrans qpi (sHeqTransport e (sPair A2' B2' tu2 tv2))).
+      destruct hu1' as [[[? ?] ?] ?].
+      destruct htu2 as [[[? ?] ?] ?].
+      destruct hv1' as [[[? ?] ?] ?].
+      destruct htv2 as [[[? ?] ?] ?].
+      destruct hA1' as [[[? ?] ?] ?].
+      destruct hA2' as [[[? ?] ?] ?].
+      destruct hB1' as [[[? ?] ?] ?].
+      destruct hB2' as [[[? ?] ?] ?].
+      repeat split.
+      * assumption.
+      * constructor ; assumption.
+      * constructor ; assumption.
+      * constructor ; assumption.
+      * constructor. constructor ; assumption.
+      * eapply type_HeqTrans' ; try eassumption.
+        eapply type_HeqTransport' ; try assumption.
+        -- eapply type_Pair' ; eassumption.
+        -- eapply type_HeqTypeEq' ; try assumption.
+           ++ eapply type_HeqSym' ; eassumption.
+           ++ eapply type_Sum ; eassumption.
 
     (* cong_Pi1 *)
     + (* The domains *)
