Translation/Equality.v
@@ -33,6 +33,7 @@ Inductive nlterm : Type :=
 | nlCongLambda (B1 B2 t1 t2 pA pB pt : nlterm)
 | nlCongApp (B1 B2 pu pA pB pv : nlterm)
 | nlCongSum (B1 B2 pA pB : nlterm)
+| nlCongPair (B1 B2 pA pB pu pv : nlterm)
 | nlCongPi1 (B1 B2 pA pB pp : nlterm)
 | nlCongPi2 (B1 B2 pA pB pp : nlterm)
 | nlCongEq (pA pu pv : nlterm)
@@ -73,6 +74,8 @@ Fixpoint nl (t : sterm) : nlterm :=
   | sCongApp B1 B2 pu pA pB pv =>
     nlCongApp (nl B1) (nl B2) (nl pu) (nl pA) (nl pB) (nl pv)
   | sCongSum B1 B2 pA pB => nlCongSum (nl B1) (nl B2) (nl pA) (nl pB)
+  | sCongPair B1 B2 pA pB pu pv =>
+    nlCongPair (nl B1) (nl B2) (nl pA) (nl pB) (nl pu) (nl pv)
   | sCongPi1 B1 B2 pA pB pp => nlCongPi1 (nl B1) (nl B2) (nl pA) (nl pB) (nl pp)
   | sCongPi2 B1 B2 pA pB pp => nlCongPi2 (nl B1) (nl B2) (nl pA) (nl pB) (nl pp)
   | sCongEq pA pu pv => nlCongEq (nl pA) (nl pu) (nl pv)
